

MATH 416 Abstract Linear Algebra

Week 15 - Homework 10

Assigned: Wed. Dec. 3, 2025

Due: Wed. Dec. 10, 2025 (by 11:59pm)

Reminder: I encourage you to work together and use resources as needed. Please remember to state who you collaborated with and what resources you used.

Exercise 1 (6 points): Trace

- (i) Prove that the trace is linear (i.e $\text{tr}[A + B] = \text{tr}[A] + \text{tr}[B]$ and $\text{tr}[zA] = z \text{tr}[A]$).

Proof. To prove linearity, it suffices to show that $\text{tr}(\alpha A + \beta B) = \alpha \text{tr}(A) + \beta \text{tr}(B)$ for any scalars α, β and $n \times n$ matrices A, B . By the definitions of scalar multiplication and matrix addition, the diagonal entry $(\alpha A + \beta B)_{ii}$ is equal to $\alpha A_{ii} + \beta B_{ii}$. Using the definition of the trace:

$$\begin{aligned}\text{tr}(\alpha A + \beta B) &= \sum_{i=1}^n (\alpha A + \beta B)_{ii} \\ &= \sum_{i=1}^n (\alpha A_{ii} + \beta B_{ii}) \\ &= \alpha \sum_{i=1}^n A_{ii} + \beta \sum_{i=1}^n B_{ii} \\ &= \alpha \text{tr}(A) + \beta \text{tr}(B).\end{aligned}$$

Thus, the trace is a linear map. □

- (ii) Show that the space of traceless matrices, $\{A \in M_n(\mathbb{F}) : \text{tr}(A) = 0\}$, is a subspace of $M_n(\mathbb{F})$. What is its dimension?

Proof. Let $W = \{A \in M_n(\mathbb{F}) : \text{tr}(A) = 0\}$ be the set of traceless matrices. First, the zero matrix 0_n is in W since $\text{tr}(0_n) = 0$. Next, we show closure under linear combinations. Let $A, B \in W$ and let α, β be scalars. By the linearity of the trace:

$$\text{tr}(\alpha A + \beta B) = \alpha \text{tr}(A) + \beta \text{tr}(B) = \alpha(0) + \beta(0) = 0.$$

Thus, $\alpha A + \beta B \in W$, so W is a subspace of $M_n(\mathbb{F})$. The space $M_n(\mathbb{F})$ has dimension n^2 . The condition $\text{tr}(A) = 0$ imposes exactly one linear constraint on the n^2 entries (specifically, the sum of the n diagonal entries must be zero). Subtracting this single

constraint from the total dimension gives:

$$\dim(W) = n^2 - 1.$$

□

(iii) Suppose V is an inner product space and $T \in \mathcal{L}(V)$. Prove that $\operatorname{tr} T^* = \overline{\operatorname{tr} T}$.

Hint: use Axler 8.55 in the fourth edition.

Proof. Let e_1, \dots, e_n be an orthonormal basis of V . By Axler 8.55 (4th ed.), the trace of an operator on an inner product space is given by:

$$\operatorname{tr}(T) = \sum_{j=1}^n \langle Te_j, e_j \rangle.$$

Applying this formula to the adjoint operator T^* , we have:

$$\begin{aligned} \operatorname{tr}(T^*) &= \sum_{j=1}^n \langle T^* e_j, e_j \rangle \\ &= \sum_{j=1}^n \langle e_j, Te_j \rangle && \text{(definition of adjoint)} \\ &= \sum_{j=1}^n \overline{\langle Te_j, e_j \rangle} && \text{(conjugate symmetry of inner product)} \\ &= \overline{\sum_{j=1}^n \langle Te_j, e_j \rangle} && \text{(additivity of complex conjugation)} \\ &= \overline{\operatorname{tr}(T)}. \end{aligned}$$

□

Exercise 2 (9 points): Determinant

(i) Prove that $\det(AB) = \det(A) \det(B)$ for all 2-by-2 matrices A, B .

Proof. Let $A = \begin{pmatrix} a & b \\ c & d \end{pmatrix}$ and $B = \begin{pmatrix} e & f \\ g & h \end{pmatrix}$. First, we calculate the product of the

individual determinants:

$$\begin{aligned}\det(A) \det(B) &= (ad - bc)(eh - fg) \\ &= adeh - adfg - bceh + bcfg. \quad (*)\end{aligned}$$

Next, we compute the matrix product AB :

$$AB = \begin{pmatrix} ae + bg & af + bh \\ ce + dg & cf + dh \end{pmatrix}.$$

Now, we compute the determinant of this product matrix:

$$\begin{aligned}\det(AB) &= (ae + bg)(cf + dh) - (af + bh)(ce + dg) \\ &= (aecf + aedh + bgcf + bgdh) - (afce + afdg + bhce + bhdg).\end{aligned}$$

Since scalar multiplication is commutative (e.g., $aecf = afce$), the first and last terms inside the parentheses cancel out:

$$\begin{aligned}\det(AB) &= aedh + bgcf - afdg - bceh. \\ &= adeh - adfg - bceh + bcfg.\end{aligned}$$

Comparing this result with (*), we see that $\det(AB) = \det(A) \det(B)$. □

(ii) Consider the matrix

$$A = \begin{pmatrix} 6 & -1 \\ 2 & 3 \end{pmatrix}. \quad (1)$$

Solve the equation $\det(A - \lambda I) = 0$ to find the eigenvalues of A .

Solution.

First, we set up the characteristic equation $\det(A - \lambda I) = 0$:

$$A - \lambda I = \begin{pmatrix} 6 & -1 \\ 2 & 3 \end{pmatrix} - \begin{pmatrix} \lambda & 0 \\ 0 & \lambda \end{pmatrix} = \begin{pmatrix} 6 - \lambda & -1 \\ 2 & 3 - \lambda \end{pmatrix}.$$

Now, we compute the determinant of this matrix:

$$\begin{aligned}\det(A - \lambda I) &= (6 - \lambda)(3 - \lambda) - (-1)(2) \\ &= (18 - 6\lambda - 3\lambda + \lambda^2) + 2 \\ &= \lambda^2 - 9\lambda + 20.\end{aligned}$$

To find the eigenvalues, we set this characteristic polynomial equal to zero and solve for λ :

$$\begin{aligned}\lambda^2 - 9\lambda + 20 &= 0 \\ (\lambda - 4)(\lambda - 5) &= 0.\end{aligned}$$

Thus, the eigenvalues are $\lambda = 4$ and $\lambda = 5$.

- (iii) Let λ_1, λ_2 be two eigenvalues of a matrix A . Define the mean and the product of the eigenvalues of a 2-by-2 matrix as

$$m = \frac{1}{2} \operatorname{tr}[A] = \frac{1}{2}(\lambda_1 + \lambda_2), \quad (2)$$

$$p = \det(A) = \lambda_1 \lambda_2. \quad (3)$$

Prove that the eigenvalues of A are given as

$$\lambda_1, \lambda_2 = m \pm \sqrt{m^2 - p}. \quad (4)$$

Proof. Let $A = \begin{pmatrix} a & b \\ c & d \end{pmatrix}$. The eigenvalues are found by solving the characteristic equation $\det(A - \lambda I) = 0$. First, we compute the determinant explicitly:

$$\begin{aligned}0 &= \det \begin{pmatrix} a - \lambda & b \\ c & d - \lambda \end{pmatrix} = (a - \lambda)(d - \lambda) - bc \\ &= ad - a\lambda - d\lambda + \lambda^2 - bc \\ &= \lambda^2 - (a + d)\lambda + (ad - bc)\end{aligned}$$

We identify the terms in the coefficients: $a + d = \operatorname{tr}(A)$, $ad - bc = \det(A)$.

Using the definitions given in the problem statement ($2m = \operatorname{tr}(A)$ and $p = \det(A)$),

we substitute these into the polynomial:

$$\lambda^2 - 2m\lambda + p = 0.$$

Now we solve for λ using the quadratic formula:

$$\begin{aligned}\lambda &= \frac{-(-2m) \pm \sqrt{(-2m)^2 - 4(1)(p)}}{2} \\ &= \frac{2m \pm \sqrt{4m^2 - 4p}}{2} \\ &= \frac{2m \pm 2\sqrt{m^2 - p}}{2} \\ &= m \pm \sqrt{m^2 - p}.\end{aligned}$$

□